src/mem/Addresses/PointerArithmetic.v
@@ -1,0 +1,318 @@
+Require Import ZArith String List Lia.
+
+From ExtLib Require Import
+     Structures.Monad
+     Structures.Functor.
+
+From Mem Require Import
+  Addresses.MemoryAddress.
+
+From LLVM_Memory Require Import
+  Sizeof
+  Intptr.
+
+Import ListNotations.
+Import MonadNotation.
+    
+Module Type GEPM (Addr:ADDRESS) (ITOP : ITOP Addr) (SIZEOF:Sizeof).
+  Import Addr.
+  Import ITOP.
+  Import SIZEOF.
+
+  (** ** Get Element Pointer
+      Retrieve the address of a subelement of an indexable (i.e. aggregate) [dtyp] [t] (i.e. vector, array, struct, packed struct).
+      The [off]set parameter contains the current entry address of the aggregate structure being analyzed, while the list
+      of [dvalue] [vs] describes the indexes of interest used to access the subelement.
+      The interpretation of these values slightly depends on the type considered.
+      But essentially, for instance in a vector or an array, the head value should be an [i32] describing the index of interest.
+      The offset is therefore incremented by this index times the size of the type of elements stored. Finally, a recursive call
+      at this new offset allows for deeper unbundling of a nested structure.
+   *)
+  Fixpoint handle_gep_h (t:dtyp) (off:Z) (vs:list dvalue): err Z :=
+    match vs with
+    | v :: vs' =>
+      match v with
+      | DVALUE_I8 i =>
+        let k := unsigned i in
+        let n := BinIntDef.Z.to_nat k in
+        match t with
+        | DTYPE_Vector _ ta
+        | DTYPE_Array _ ta =>
+          handle_gep_h ta (off + k * (Z.of_N (sizeof_dtyp ta))) vs'
+        | _ => failwith ("non-i8-indexable type")
+        end
+      | DVALUE_I32 i =>
+        let k := unsigned i in
+        let n := BinIntDef.Z.to_nat k in
+        match t with
+        | DTYPE_Vector _ ta
+        | DTYPE_Array _ ta =>
+          handle_gep_h ta (off + k * (Z.of_N (sizeof_dtyp ta))) vs'
+        | DTYPE_Struct ts
+        | DTYPE_Packed_struct ts => (* Handle these differently in future *)
+          let offset := fold_left (fun acc t => (acc + (Z.of_N (sizeof_dtyp t))))%Z
+                                  (firstn n ts) 0%Z in
+          match nth_error ts n with
+          | None => failwith "overflow"
+          | Some t' =>
+            handle_gep_h t' (off + offset) vs'
+          end
+        | _ => failwith ("non-i32-indexable type")
+        end
+      | DVALUE_I64 i =>
+        let k := unsigned i in
+        let n := BinIntDef.Z.to_nat k in
+        match t with
+        | DTYPE_Vector _ ta
+        | DTYPE_Array _ ta =>
+          handle_gep_h ta (off + k * (Z.of_N (sizeof_dtyp ta))) vs'
+        | _ => failwith ("non-i64-indexable type")
+        end
+      | DVALUE_IPTR i =>
+        let k := IP.to_Z i in
+        let n := BinIntDef.Z.to_nat k in
+        match t with
+        | DTYPE_Vector _ ta
+        | DTYPE_Array _ ta =>
+          handle_gep_h ta (off + k * (Z.of_N (sizeof_dtyp ta))) vs'
+        | _ => failwith ("non-iptr-indexable type")
+        end
+      | _ => failwith "handle_gep_h: unsupported index type"
+      end
+    | [] => ret off
+    end.
+
+  (* At the toplevel, GEP takes a [dvalue] as an argument that must contain a pointer, but no other pointer can be recursively followed.
+     The pointer set the block into which we look, and the initial offset. The first index value add to the initial offset passed to [handle_gep_h] for the actual access to structured data.
+   *)
+  Definition handle_gep_addr (t:dtyp) (a:addr) (vs:list dvalue) : err (OOM addr) :=
+    let ptr := ptr_to_int a in
+    let prov := address_provenance a in
+    match vs with
+    | DVALUE_I8 i :: vs' =>
+      ptr' <- handle_gep_h t (ptr + Z.of_N (sizeof_dtyp t) * (unsigned i)) vs' ;;
+      ret (int_to_ptr ptr' prov)
+    | DVALUE_I32 i :: vs' =>
+      ptr' <- handle_gep_h t (ptr + Z.of_N (sizeof_dtyp t) * (unsigned i)) vs' ;;
+      ret (int_to_ptr ptr' prov)
+    | DVALUE_I64 i :: vs' =>
+      ptr' <- handle_gep_h t (ptr + Z.of_N (sizeof_dtyp t) * (unsigned i)) vs' ;;
+      ret (int_to_ptr ptr' prov)
+    | DVALUE_IPTR i :: vs' =>
+      ptr' <- handle_gep_h t (ptr + Z.of_N (sizeof_dtyp t) * (IP.to_Z i)) vs' ;;
+      ret (int_to_ptr ptr' prov)
+    | [] => failwith "handle_gep_addr: no indices"
+    | _ => failwith "handle_gep_addr: unsupported index type"
+    end.
+
+  Lemma handle_gep_addr_0 :
+    forall (dt : dtyp) (p : addr),
+      handle_gep_addr dt p [DVALUE_IPTR IP.zero] = inr (ret p).
+  Proof.
+    intros dt p.
+    cbn.
+    rewrite IP.to_Z_0.
+    replace (ptr_to_int p + Z.of_N (sizeof_dtyp dt) * 0)%Z with (ptr_to_int p) by lia.
+    rewrite int_to_ptr_ptr_to_int; auto.
+  Qed.
+
+  Lemma handle_gep_addr_nil :
+    forall (dt : dtyp) (p : addr),
+      handle_gep_addr dt p [] = inl "handle_gep_addr: no indices"%string.
+  Proof.
+    intros dt p.
+    cbn; auto.
+  Qed.
+
+  Lemma handle_gep_addr_ix :
+    forall (dt : dtyp) (p p' : addr) ix,
+      handle_gep_addr dt p [DVALUE_IPTR ix] = inr (ret p') ->
+      ptr_to_int p' = (ptr_to_int p + Z.of_N (sizeof_dtyp dt) * IP.to_Z ix)%Z.
+  Proof.
+    intros dt p p' ix GEP.
+    cbn in *.
+    inv GEP.
+    erewrite ptr_to_int_int_to_ptr; eauto.
+  Qed.
+
+  Lemma handle_gep_addr_ix_OOM :
+    forall (dt : dtyp) (p p' : addr) ix msg,
+      handle_gep_addr dt p [DVALUE_IPTR ix] = inr (Oom msg) ->
+      exists msg',
+        int_to_ptr (ptr_to_int p + Z.of_N (sizeof_dtyp dt) * IP.to_Z ix)%Z (address_provenance p) = Oom msg'.
+  Proof.
+    intros dt p p' ix msg GEP.
+    cbn in *.
+    exists msg.
+    inv GEP.
+    auto.
+  Qed.
+
+  Lemma handle_gep_addr_ix' :
+    forall (dt : dtyp) (p p' : addr) ix,
+      ret p' = int_to_ptr (ptr_to_int p + Z.of_N (sizeof_dtyp dt) * IP.to_Z ix)%Z (address_provenance p) ->
+      handle_gep_addr dt p [DVALUE_IPTR ix] = inr (ret p').
+  Proof.
+    intros dt p p' ix IX.
+    cbn in *.
+    inv IX.
+    reflexivity.
+  Qed.
+
+  Lemma handle_gep_addr_ix'_OOM :
+    forall (dt : dtyp) (p p' : addr) ix msg,
+      int_to_ptr (ptr_to_int p + Z.of_N (sizeof_dtyp dt) * IP.to_Z ix)%Z (address_provenance p) = Oom msg ->
+      exists msg', handle_gep_addr dt p [DVALUE_IPTR ix] = inr (Oom msg').
+  Proof.
+    intros dt p p' ix msg IX.
+    cbn in *.
+    exists msg.
+    inv IX.
+    auto.
+  Qed.
+
+  (* Lemma handle_gep_addr_cons_inv : *)
+  (*   forall t base_addr idx idxs final_addr, *)
+  (*     handle_gep_addr t base_addr (idx :: idxs) = inr (ret final_addr) -> *)
+  (*     exists res_addr, *)
+  (*       handle_gep_addr t base_addr [idx] = inr (ret res_addr) /\ *)
+  (*         handle_gep_addr t res_addr idxs = inr (ret res_addr). *)
+  (* Proof. *)
+  (*   intros t base_addr idx idxs final_addr H. *)
+  (*   cbn in H. *)
+  (*   break_match_hyp_inv. *)
+  (*   - break_match_hyp_inv. *)
+  (*     exists final_addr. *)
+
+
+  (*     remember (int_to_ptr (ptr_to_int base_addr + Z.of_N (sizeof_dtyp t) * DynamicValues.Int8.unsigned x) (address_provenance base_addr)). *)
+  (*     pose proof int_to_ptr_ptr_to_int_exists. *)
+  (*     exists (int_to_ptr (ptr_to_int base_addr + Z.of_N (sizeof_dtyp t) * DynamicValues.Int8.unsigned x) (address_provenance base_addr)). *)
+
+  (* Qed. *)
+
+  (* Lemma handle_gep_h_cons : *)
+  (*   forall idxs idx t base_addr res_addr final_addr, *)
+  (*     handle_gep_h t base_addr [idx] = inr res_addr -> *)
+  (*     handle_gep_h t res_addr idxs = inr final_addr -> *)
+  (*     handle_gep_h t base_addr (idx :: idxs) = inr final_addr. *)
+  (* Proof. *)
+  (*   intros idxs. *)
+  (*   induction idxs; intros idx t base_addr res_addr final_addr GEP_START GEP_REST. *)
+  (*   - cbn in GEP_REST. inv GEP_REST; auto. *)
+  (*   - specialize  *)
+  (*     cbn in GEP_REST. *)
+  (*     break_match_hyp_inv. *)
+  (*     + break_match_hyp_inv. *)
+  (*       specialize x (res_addr + DynamicValues.Int8.unsigned x * Z.of_N (sizeof_dtyp d)) *)
+  (*       * cbn in H1. *)
+
+  (*     specialize (IHidxs a t res_addr). *)
+      
+      
+  (*   cbn; cbn in GEP_START. *)
+  (*   break_match_hyp_inv. *)
+  (*   - break_match_hyp_inv. *)
+  (*     + generalize dependent final_addr. *)
+  (*       generalize dependent base_addr. *)
+  (*       induction idxs; intros base_addr final_addr GEP_REST. *)
+  (*       * cbn in *; auto. *)
+  (*       * cbn in *. *)
+  (*         break_match_hyp_inv. *)
+  (*         --  *)
+  (* Qed. *)
+
+  (* Lemma handle_gep_addr_cons : *)
+  (*   forall idx idxs t base_addr res_addr final_addr, *)
+  (*     handle_gep_addr t base_addr [idx] = inr (ret res_addr) -> *)
+  (*     handle_gep_addr t res_addr idxs = inr (ret final_addr) -> *)
+  (*     handle_gep_addr t base_addr (idx :: idxs) = inr (ret final_addr). *)
+  (* Proof. *)
+  (*   intros idx. *)
+  (*   induction idxs; intros t base_addr res_addr final_addr GEP_START GEP_REST. *)
+  (*   - cbn in GEP_REST. inv GEP_REST. *)
+  (*   - cbn in GEP_START. *)
+  (*     cbn. *)
+  (*     break_match_hyp_inv. *)
+  (*     + cbn in GEP_REST. *)
+  (*       break_match_hyp_inv. *)
+  (*       * break_match_hyp_inv. *)
+  (*         break_match_goal. *)
+  (*         admit. *)
+
+  (*         break_match_hyp_inv. *)
+          
+      
+
+  (*   intros t base_addr idx idxs res_addr final_addr GEP_START GEP_REST. *)
+  (*   cbn. *)
+  (*   cbn in GEP_START. *)
+  (*   break_match_hyp_inv. *)
+  (*   - unfold handle_gep_addr in GEP_REST. *)
+  (*     induction idxs; inv GEP_REST. *)
+  (*     forward IHidxs. *)
+      
+      
+  (*     generalize dependent res_addr. *)
+  (*     induction idxs; intros res_addr GEP_REST H0. *)
+  (*     + inv GEP_REST. *)
+  (*     + cbn. *)
+  (*       setoid_rewrite GEP_REST. *)
+  (*     break_match_goal. *)
+  (*     + unfold handle_gep_addr in GEP_REST. *)
+  (*       break_match_hyp_inv. *)
+  (*       break_match_hyp_inv. *)
+  (*       cbn in *. *)
+  (*       break_match_hyp_inv. *)
+  (*       break_match_hyp_inv. *)
+
+                             
+        
+  (*   reflexivity. *)
+  (* Qed. *)
+
+  Lemma handle_gep_addr_preserves_provenance :
+    forall (dt : dtyp) ixs (p p' : addr),
+      handle_gep_addr dt p ixs = inr (ret p') ->
+      address_provenance p = address_provenance p'.
+  Proof.
+    intros dt ixs.
+    induction ixs;
+      intros p p' GEP;
+      [inversion GEP|].
+
+    cbn in GEP.
+    destruct a; inversion GEP.
+    - break_match_hyp; inv GEP.
+      cbn in *.
+      symmetry.
+      eapply int_to_ptr_provenance; eauto.
+    - break_match_hyp; inv GEP.
+      symmetry.
+      eapply int_to_ptr_provenance; eauto.
+    - break_match_hyp; inv GEP.
+      symmetry.
+      eapply int_to_ptr_provenance; eauto.
+    - break_match_hyp; inv GEP.
+      symmetry.
+      eapply int_to_ptr_provenance; eauto.
+  Qed.
+
+  Definition handle_gep (t:dtyp) (dv:dvalue) (vs:list dvalue) : err (OOM dvalue) :=
+    match dv with
+    | DVALUE_Addr a => fmap (F:=err) (fmap DVALUE_Addr) (handle_gep_addr t a vs)
+    | _ => inl "non-address"%string
+    end.
+End GEPM.
+
+Module Make (ADDR : ADDRESS) (IP : INTPTR) (SIZE : Sizeof) (Events : LLVM_INTERACTIONS(ADDR)(IP)(SIZE)) (PTOI : PTOI ADDR) (PROV : PROVENANCE ADDR) (ITOP : ITOP ADDR PROV PTOI) <: GEPM(ADDR)(PTOI)(PROV)(ITOP)(IP)(SIZE)(Events).
+  Import ADDR.
+  Import Events.
+  Import DV.
+  Import SIZE.
+  Import PTOI.
+  Import ITOP.
+  Import PROV.
+
+  Include GEPM (ADDR)(PTOI)(PROV)(ITOP)(IP)(SIZE)(Events).
+End Make.
