src/mem/MemPropT.v
@@ -21,12 +21,9 @@ From Vellvm.Utils Require Import
      Tactics
      Inhabited.
 
-From Vellvm.Handlers.MemoryModules Require Import
-     Within.
-
-From Vellvm.Semantics Require Import
-  StoreId
-  LLVMEvents.
+From Mem Require Import
+  MemoryModules.Within
+  Semantics.Memory.StoreId.
 
 Import Basics.Basics.Monads.
 Import MonadNotation.
@@ -528,26 +525,3 @@ Definition MemPropT_assert_pre {MemState} (assertion : Prop) : MemPropT MemState
                ms = ms' /\ assertion
            end
        end.
-
-Definition MemPropT_lift_PropT {MemState X} {E} `{UBE -< E} `{OOME -< E} `{FailureE -< E} (spec : MemPropT MemState X) :
-  stateT MemState (PropT E) X.
-Proof.
-  unfold PropT, MemPropT, stateT in *.
-  refine
-    (fun ms t =>
-       (* UB *)
-       (exists msg_spec,
-           spec ms (raise_ub msg_spec)) \/
-         (* Error *)
-         ((exists msg,
-              t ≈ (raise_error msg) /\
-              exists msg_spec, spec ms (raise_error msg_spec))) \/
-           (* OOM *)
-           (exists msg,
-               t ≈ (raise_oom msg) /\
-               exists msg_spec, spec ms (raise_oom msg_spec)) \/
-           (* Success *)
-           (exists ms' x,
-               t ≈ (ret (ms', x)) /\
-               spec ms (ret (ms', x)))).
-Defined.
