src/mem/SByte.v
@@ -1,0 +1,7 @@
+From Mem Require Import
+  StoreId.
+
+Module Type SBYTE.
+Parameter SByte : Type.
+Parameter sbyte_sid : SByte -> store_id.
+End SBYTE.
